examples/OCL_lib_Gogolla_challenge_integer.thy
@@ -57,47 +57,47 @@ lemma including_swap_ :
      and i_val : "\<tau> \<Turnstile> \<upsilon> i"
      and j_val : "\<tau> \<Turnstile> \<upsilon> j"
    shows "\<tau> \<Turnstile> ((S :: ('\<AA>, int option option) Set)->including(i)->including(j) \<doteq> (S->including(j)->including(i)))"
-by(rule including_swap__generic[OF includes_execute_int StrictRefEq\<^sub>I\<^sub>n\<^sub>t\<^sub>e\<^sub>g\<^sub>e\<^sub>r_refl StrictRefEq\<^sub>I\<^sub>n\<^sub>t\<^sub>e\<^sub>g\<^sub>e\<^sub>r_defined_args_valid including_includes], simp_all add: assms)
+by(rule including_swap__generic[OF OclIncludes_execute\<^sub>I\<^sub>n\<^sub>t\<^sub>e\<^sub>g\<^sub>e\<^sub>r StrictRefEq\<^sub>I\<^sub>n\<^sub>t\<^sub>e\<^sub>g\<^sub>e\<^sub>r_refl StrictRefEq\<^sub>I\<^sub>n\<^sub>t\<^sub>e\<^sub>g\<^sub>e\<^sub>r_defined_args_valid OclIncludes_including\<^sub>I\<^sub>n\<^sub>t\<^sub>e\<^sub>g\<^sub>e\<^sub>r], simp_all add: assms)
 
 lemma including_swap' : "\<tau> \<Turnstile> \<delta> S \<Longrightarrow> \<tau> \<Turnstile> \<upsilon> i \<Longrightarrow> \<tau> \<Turnstile> \<upsilon> j \<Longrightarrow> ((S :: ('\<AA>, int option option) Set)->including(i)->including(j) \<tau> = (S->including(j)->including(i)) \<tau>)"
-by(rule including_swap'_generic[OF including_swap_0_generic[OF includes_execute_int StrictRefEq\<^sub>I\<^sub>n\<^sub>t\<^sub>e\<^sub>g\<^sub>e\<^sub>r_refl StrictRefEq\<^sub>I\<^sub>n\<^sub>t\<^sub>e\<^sub>g\<^sub>e\<^sub>r_defined_args_valid including_includes]])
+by(rule including_swap'_generic[OF including_swap_0_generic[OF OclIncludes_execute\<^sub>I\<^sub>n\<^sub>t\<^sub>e\<^sub>g\<^sub>e\<^sub>r StrictRefEq\<^sub>I\<^sub>n\<^sub>t\<^sub>e\<^sub>g\<^sub>e\<^sub>r_refl StrictRefEq\<^sub>I\<^sub>n\<^sub>t\<^sub>e\<^sub>g\<^sub>e\<^sub>r_defined_args_valid OclIncludes_including\<^sub>I\<^sub>n\<^sub>t\<^sub>e\<^sub>g\<^sub>e\<^sub>r]])
 
 lemma including_swap : "\<forall>\<tau>. \<tau> \<Turnstile> \<delta> S \<Longrightarrow> \<forall>\<tau>. \<tau> \<Turnstile> \<upsilon> i \<Longrightarrow> \<forall>\<tau>. \<tau> \<Turnstile> \<upsilon> j \<Longrightarrow> ((S :: ('\<AA>, int option option) Set)->including(i)->including(j) = (S->including(j)->including(i)))"
-by(rule including_swap_generic[OF including_swap_0_generic[OF includes_execute_int StrictRefEq\<^sub>I\<^sub>n\<^sub>t\<^sub>e\<^sub>g\<^sub>e\<^sub>r_refl StrictRefEq\<^sub>I\<^sub>n\<^sub>t\<^sub>e\<^sub>g\<^sub>e\<^sub>r_defined_args_valid including_includes]])
+by(rule including_swap_generic[OF including_swap_0_generic[OF OclIncludes_execute\<^sub>I\<^sub>n\<^sub>t\<^sub>e\<^sub>g\<^sub>e\<^sub>r StrictRefEq\<^sub>I\<^sub>n\<^sub>t\<^sub>e\<^sub>g\<^sub>e\<^sub>r_refl StrictRefEq\<^sub>I\<^sub>n\<^sub>t\<^sub>e\<^sub>g\<^sub>e\<^sub>r_defined_args_valid OclIncludes_including\<^sub>I\<^sub>n\<^sub>t\<^sub>e\<^sub>g\<^sub>e\<^sub>r]])
 
 section{* Properties: (with comp fun commute) OclIncluding *}
 subsection{* Preservation of comp fun commute (instance) *}
 
 lemma including_commute : "EQ_comp_fun_commute (\<lambda>j (r2 :: ('\<AA>, int option option) Set). (r2->including(j)))"
-by(rule including_commute_generic[OF including_swap'_generic[OF including_swap_0_generic[OF includes_execute_int StrictRefEq\<^sub>I\<^sub>n\<^sub>t\<^sub>e\<^sub>g\<^sub>e\<^sub>r_refl StrictRefEq\<^sub>I\<^sub>n\<^sub>t\<^sub>e\<^sub>g\<^sub>e\<^sub>r_defined_args_valid including_includes]]])
+by(rule including_commute_generic[OF including_swap'_generic[OF including_swap_0_generic[OF OclIncludes_execute\<^sub>I\<^sub>n\<^sub>t\<^sub>e\<^sub>g\<^sub>e\<^sub>r StrictRefEq\<^sub>I\<^sub>n\<^sub>t\<^sub>e\<^sub>g\<^sub>e\<^sub>r_refl StrictRefEq\<^sub>I\<^sub>n\<^sub>t\<^sub>e\<^sub>g\<^sub>e\<^sub>r_defined_args_valid OclIncludes_including\<^sub>I\<^sub>n\<^sub>t\<^sub>e\<^sub>g\<^sub>e\<^sub>r]]])
 
 lemma including_commute2 :
  assumes i_int : "is_int i"
    shows "EQ_comp_fun_commute (\<lambda>x (acc :: ('\<AA>, int option option) Set). ((acc->including(x))->including(i)))"
-by(rule including_commute2_generic[OF including_swap'_generic[OF including_swap_0_generic[OF includes_execute_int StrictRefEq\<^sub>I\<^sub>n\<^sub>t\<^sub>e\<^sub>g\<^sub>e\<^sub>r_refl StrictRefEq\<^sub>I\<^sub>n\<^sub>t\<^sub>e\<^sub>g\<^sub>e\<^sub>r_defined_args_valid including_includes]]], simp_all add: assms)
+by(rule including_commute2_generic[OF including_swap'_generic[OF including_swap_0_generic[OF OclIncludes_execute\<^sub>I\<^sub>n\<^sub>t\<^sub>e\<^sub>g\<^sub>e\<^sub>r StrictRefEq\<^sub>I\<^sub>n\<^sub>t\<^sub>e\<^sub>g\<^sub>e\<^sub>r_refl StrictRefEq\<^sub>I\<^sub>n\<^sub>t\<^sub>e\<^sub>g\<^sub>e\<^sub>r_defined_args_valid OclIncludes_including\<^sub>I\<^sub>n\<^sub>t\<^sub>e\<^sub>g\<^sub>e\<^sub>r]]], simp_all add: assms)
 
 lemma including_commute3 :
  assumes i_int : "is_int i"
    shows "EQ_comp_fun_commute (\<lambda>x (acc :: ('\<AA>, int option option) Set). acc->including(i)->including(x))"
-by(rule including_commute3_generic[OF including_swap'_generic[OF including_swap_0_generic[OF includes_execute_int StrictRefEq\<^sub>I\<^sub>n\<^sub>t\<^sub>e\<^sub>g\<^sub>e\<^sub>r_refl StrictRefEq\<^sub>I\<^sub>n\<^sub>t\<^sub>e\<^sub>g\<^sub>e\<^sub>r_defined_args_valid including_includes]]], simp_all add: assms)
+by(rule including_commute3_generic[OF including_swap'_generic[OF including_swap_0_generic[OF OclIncludes_execute\<^sub>I\<^sub>n\<^sub>t\<^sub>e\<^sub>g\<^sub>e\<^sub>r StrictRefEq\<^sub>I\<^sub>n\<^sub>t\<^sub>e\<^sub>g\<^sub>e\<^sub>r_refl StrictRefEq\<^sub>I\<^sub>n\<^sub>t\<^sub>e\<^sub>g\<^sub>e\<^sub>r_defined_args_valid OclIncludes_including\<^sub>I\<^sub>n\<^sub>t\<^sub>e\<^sub>g\<^sub>e\<^sub>r]]], simp_all add: assms)
 
 lemma including_commute4 :
  assumes i_int : "is_int i"
      and j_int : "is_int j"
    shows "EQ_comp_fun_commute (\<lambda>x (acc :: ('\<AA>, int option option) Set). acc->including(i)->including(x)->including(j))"
-by(rule including_commute4_generic[OF including_swap'_generic[OF including_swap_0_generic[OF includes_execute_int StrictRefEq\<^sub>I\<^sub>n\<^sub>t\<^sub>e\<^sub>g\<^sub>e\<^sub>r_refl StrictRefEq\<^sub>I\<^sub>n\<^sub>t\<^sub>e\<^sub>g\<^sub>e\<^sub>r_defined_args_valid including_includes]]], simp_all add: assms)
+by(rule including_commute4_generic[OF including_swap'_generic[OF including_swap_0_generic[OF OclIncludes_execute\<^sub>I\<^sub>n\<^sub>t\<^sub>e\<^sub>g\<^sub>e\<^sub>r StrictRefEq\<^sub>I\<^sub>n\<^sub>t\<^sub>e\<^sub>g\<^sub>e\<^sub>r_refl StrictRefEq\<^sub>I\<^sub>n\<^sub>t\<^sub>e\<^sub>g\<^sub>e\<^sub>r_defined_args_valid OclIncludes_including\<^sub>I\<^sub>n\<^sub>t\<^sub>e\<^sub>g\<^sub>e\<^sub>r]]], simp_all add: assms)
 
 lemma including_commute5 :
  assumes i_int : "is_int i"
      and j_int : "is_int j"
    shows "EQ_comp_fun_commute (\<lambda>x (acc :: ('\<AA>, int option option) Set). acc->including(x)->including(j)->including(i))"
-by(rule including_commute5_generic[OF including_swap'_generic[OF including_swap_0_generic[OF includes_execute_int StrictRefEq\<^sub>I\<^sub>n\<^sub>t\<^sub>e\<^sub>g\<^sub>e\<^sub>r_refl StrictRefEq\<^sub>I\<^sub>n\<^sub>t\<^sub>e\<^sub>g\<^sub>e\<^sub>r_defined_args_valid including_includes]]], simp_all add: assms)
+by(rule including_commute5_generic[OF including_swap'_generic[OF including_swap_0_generic[OF OclIncludes_execute\<^sub>I\<^sub>n\<^sub>t\<^sub>e\<^sub>g\<^sub>e\<^sub>r StrictRefEq\<^sub>I\<^sub>n\<^sub>t\<^sub>e\<^sub>g\<^sub>e\<^sub>r_refl StrictRefEq\<^sub>I\<^sub>n\<^sub>t\<^sub>e\<^sub>g\<^sub>e\<^sub>r_defined_args_valid OclIncludes_including\<^sub>I\<^sub>n\<^sub>t\<^sub>e\<^sub>g\<^sub>e\<^sub>r]]], simp_all add: assms)
 
 lemma including_commute6 :
  assumes i_int : "is_int i"
      and j_int : "is_int j"
    shows "EQ_comp_fun_commute (\<lambda>x (acc :: ('\<AA>, int option option) Set). acc->including(i)->including(j)->including(x))"
-by(rule including_commute6_generic[OF including_swap'_generic[OF including_swap_0_generic[OF includes_execute_int StrictRefEq\<^sub>I\<^sub>n\<^sub>t\<^sub>e\<^sub>g\<^sub>e\<^sub>r_refl StrictRefEq\<^sub>I\<^sub>n\<^sub>t\<^sub>e\<^sub>g\<^sub>e\<^sub>r_defined_args_valid including_includes]]], simp_all add: assms)
+by(rule including_commute6_generic[OF including_swap'_generic[OF including_swap_0_generic[OF OclIncludes_execute\<^sub>I\<^sub>n\<^sub>t\<^sub>e\<^sub>g\<^sub>e\<^sub>r StrictRefEq\<^sub>I\<^sub>n\<^sub>t\<^sub>e\<^sub>g\<^sub>e\<^sub>r_refl StrictRefEq\<^sub>I\<^sub>n\<^sub>t\<^sub>e\<^sub>g\<^sub>e\<^sub>r_defined_args_valid OclIncludes_including\<^sub>I\<^sub>n\<^sub>t\<^sub>e\<^sub>g\<^sub>e\<^sub>r]]], simp_all add: assms)
 
 section{* Properties: (with comp fun commute) OclIterate and OclIncluding *}
 subsection{* Identity *}
